# 2. Classification

## Q 20

Take any $x \in \mathbb{R}^{p}$. What we need to show is that for each $y \in \{1, -1\}$,
$$
P(Y = y) = \frac{1}{1 + \exp(-y(\beta_{0} + \beta^{T}x))}
$$
holds.

When $y=1$,
$$
\begin{aligned}
\frac{1}{1 + \exp(-y(\beta_{0} + \beta^{T}x))} 
&= \frac{1}{1 + \exp(-(\beta_{0} + \beta^{T}x))} \\
&= \frac{\exp(\beta_{0} + \beta^{T}x)}{[1 + \exp(-(\beta_{0} + \beta^{T}x))]\exp(\beta_{0} + \beta^{T}x)} \\
&= \frac{\exp(\beta_{0} + \beta^{T}x)}{\exp(\beta_{0} + \beta^{T}x) + 1} \\
&= P(Y = 1).
\end{aligned}
$$

When $y=-1$,
$$
\begin{aligned}
\frac{1}{1 + \exp(-y(\beta_{0} + \beta^{T}x))} 
&= \frac{1}{1 + \exp(\beta_{0} + \beta^{T}x)} \\
&= P(Y = -1),
\end{aligned}
$$
which completes the proof.

## Q 21

Taking the derivative of $f$,
$$
\begin{aligned}
f^{\prime}(x) &= \frac{\beta \exp(- \beta_{0} - \beta x)}{[1 + \exp(- \beta_{0} - \beta x)]^{2}} \\
&= \beta \frac{\exp(- \beta_{0} - \beta x)}{1 + \exp(- \beta_{0} - \beta x)}  \cdot \frac{1}{1 + \exp(- \beta_{0} - \beta x)} \\
&= \beta \frac{\exp(- \beta_{0} - \beta x)}{1 + \exp(- \beta_{0} - \beta x)}  \cdot f(x) \\
&= \beta \frac{1 + \exp(- \beta_{0} - \beta x) - 1}{1 + \exp(- \beta_{0} - \beta x)}  \cdot f(x) \\
&= \beta \left(1 - \frac{1}{1 + \exp(- \beta_{0} - \beta x)} \right) f(x) \\
&= \beta \left(1 - f(x) \right)  f(x) \\
&= \beta f(x) \left(1 - f(x) \right) \\
\end{aligned}
$$
Since $f(x) > 0$ for all $x \in \mathbb{R}$, $f^{\prime}(x) > 0$ for all $x \in \mathbb{R}$. Thus $f$ is monotonically increasing.

Let $A := 1 + \exp(- \beta_{0} - \beta x)$. Using the result above,
$$
\begin{aligned}
\frac{f^{\prime\prime}(x)}{\beta} &= f^{\prime}(x) \left(1 - f(x) \right) + f(x) (-f^{\prime}(x)) \\
&= \beta f(x) \left(1 - f(x) \right)^{2} - \beta [f(x)]^{2} \left(1 - f(x) \right) \\
&= \beta f(x) \left(1 - f(x) \right)(1 - f(x) - f(x)) \\
&= f^{\prime}(x)(1 - 2f(x)) \\
&= f^{\prime}(x) \left[1 - \frac{2}{1 + \exp(- \beta_{0} - \beta x)} \right] \\
&= f^{\prime}(x) \left[\frac{\exp(- \beta_{0} - \beta x) - 1}{1 + \exp(- \beta_{0} - \beta x)} \right] \\
&= \frac{f^{\prime}(x)}{f(x)}[\exp(- \beta_{0} - \beta x) - 1] \\
\therefore f^{\prime\prime}(x) &= \beta \frac{f^{\prime}(x)}{f(x)}[\exp(- \beta_{0} - \beta x) - 1] 
\end{aligned}
$$

Note that $\beta \frac{f^{\prime}(x)}{f(x)} > 0$. Thus $f(x)$ is convex if and only if:
$$
\begin{aligned}
f^{\prime\prime}(x) > 0 &\Leftrightarrow \exp(-\beta_{0} - \beta x) - 1 > 0 \\
&\Leftrightarrow \exp(-\beta_{0} - \beta x) > 1 \\
&\Leftrightarrow -\beta_{0} - \beta x > 0 \\
&\Leftrightarrow x < - \frac{\beta_{0}}{\beta}.
\end{aligned}
$$

Analogously, we can show that $f(x)$ is concave if and only if:
$$
\begin{aligned}
f^{\prime\prime}(x) < 0 &\Leftrightarrow x >- \frac{\beta_{0}}{\beta}.
\end{aligned}
$$

```{r}
# Define a function
logit <- function(x, beta = 1, beta_0 = 0){
  output <- exp(beta_0 + beta * x) / (1 + exp(beta_0 +beta * x))
  return(output)
}
# Plot the function for each beta
beta_seq_expand <- expand.grid(b = seq(0, 10, by = .5))
g_21 <- ggplot(data.frame(X = c(-10, 10)), aes(x = X)) +
  mapply(
    function(b, co) stat_function(fun = logit, args = list(beta = b), aes_q(color = co)),
    beta_seq_expand$b, beta_seq_expand$b
  ) +
  ggtitle("Logistics curve") +
  labs(color = latex2exp::TeX("$\\beta$"))
plot(g_21)
```


